Some progress? Just this lemma now...

examples/lists/list-utils.dfy
@@ -103,36 +103,8 @@ module Lists {
     case Cons(a, x) => Conc(El(a), SimpleCoding(x))
   }
 
-  // function method Aux(orig: List, right: List, x: ListC, a: int, y: ListC): set<ListC> 
-  //   decreases y 
-  //   requires SimpleCoding(right) == Conc(El(a), y) 
-  //   requires Rep(AssociateRight(x, a, y)) == orig
-  //   requires y != NilC ==> y.Conc? 
-  //   requires y != NilC ==> y.left.El? // specifies the structure of y
-  //   requires x.Conc? ==> InitDecomposableC(x)
-  //   requires x == NilC ==> Conc(El(a), y) == SimpleCoding(orig)
-  //   ensures forall t: ListC :: (t in Aux(orig, right, x, a, y)) ==> t.Conc?
-  //   ensures forall t: ListC :: (t in Aux(orig, right, x, a, y)) ==> (t.left.Conc? ==> InitDecomposableC(t.left))
-  //   ensures forall t: ListC :: (t in Aux(orig, right, x, a, y)) ==> t.left != NilC
-  //   ensures AssociateLeft(x, a, y) in Aux(orig, right, x, a, y) ==> AssociateRight(x, a, y) in Aux(orig, right, x, a, y)
-  //   ensures Rep(AssociateRight(x, a, y)) == orig
-  // {
-  //   RepInvariant(x, a, y);
-  //   // assume Rep(AssociateRight(x, a, y)) == orig;
-  //   if y == NilC then {AssociateRight(x, a, y)}
-  //                else Aux(orig, right.tail, if x == NilC then El(a) else Conc(x, El(a)), y.left.val, y.right) + {AssociateRight(x, a, y)}
-  // }
 
-  // function method ComplexCoding(l: List): set<ListC>
-  //   ensures l != Nil ==> forall t: ListC :: t in ComplexCoding(l) ==> t.Conc?
-  //   ensures l != Nil ==> forall t: ListC :: (t in ComplexCoding(l) && t.Conc? && t.left.Conc?) ==> InitDecomposableC(t.left)
-  //   // ensures forall x: ListC, a: int, y: ListC :: AssociateLeft(x, a, y) in ComplexCoding(l) ==> AssociateRight(x, a, y) in ComplexCoding(l)
-  // {
-  //   assume l.Cons? ==> Rep(AssociateRight(NilC, l.head, SimpleCoding(l.tail))) == l;
-  //   if l == Nil then {NilC} else Aux(l, l, NilC, l.head, SimpleCoding(l.tail))
-  // }
-
-  function method NewAux(orig: List, x: ListC, y: List): set<ListC> 
+  function method NewAux(orig: List, x: ListC, y: List): seq<ListC> 
     decreases y
     requires x.El? || x.Conc?
     requires !x.Conc? ==> orig == Cons(x.val, y) // Special case
@@ -147,23 +119,25 @@ module Lists {
     ensures ListConc(Rep(x), y) == orig 
     ensures y == Nil ==> forall t: ListC :: t in NewAux(orig, x, y) ==> ListConc(Rep(t.left), Rep(t.right)) == orig 
     // ensures y != Nil ==> (NewAux(orig, x, y) - NewAux(orig, Conc(x, El(y.head)), y.tail)) == {Conc(x, SimpleCoding(y))} // maybe using a seq will be better? 
-    // ensures y != Nil ==> forall t: ListC :: t in (NewAux(orig, x, y) - NewAux(orig, Conc(x, El(y.head)), y.tail)) ==> ListConc(Rep(t.left), Rep(t.right)) == orig 
+    // ensures y != Nil ==> forall t: ListC :: (t in NewAux(orig, x, y) ==> ListConc(Rep(t.left), Rep(t.right)) == orig)
   {
     RepAssociation(x, y);
     match y 
-    case Nil => {Conc(x, NilC)} 
-    case Cons(head, tail) => NewAux(orig, Conc(x, El(head)), tail) + {Conc(x, SimpleCoding(y))}
+    case Nil => [Conc(x, NilC)]
+    case Cons(head, tail) => NewAux(orig, Conc(x, El(head)), tail) + [Conc(x, SimpleCoding(y))]
     // {Conc(Conc(x, El(head)), SimpleCoding(tail))}
     //{AssociateLeft(x, head, SimpleCoding(y))}
   }
 
-  function method NewComplex(l: List): set<ListC> 
+  function method NewComplex(l: List): seq<ListC> 
     ensures l != Nil ==> forall t: ListC :: (t in NewComplex(l) ==> t.Conc?)
     ensures l != Nil ==> forall t: ListC :: (t in NewComplex(l) && !t.left.Conc?) ==> t == SimpleCoding(l)
     // ensures l != Nil ==> forall t: ListC :: (t in NewComplex(l) && t.left.Conc?) ==> InitDecomposableC(t.left)
+    // ensures l != Nil ==> forall t: ListC :: (t in NewComplex(l) ==> ListConc(Rep(t.left), Rep(t.right)) == l)
   {
+    // AuxProperty(l, El(l.head), l.tail);
     // NewAux(NilC, l) // maybe instead El(l.head), l.tail?
-    if l == Nil then {NilC} else NewAux(l, El(l.head), l.tail)
+    if l == Nil then [NilC] else NewAux(l, El(l.head), l.tail)
   }
 
   /**** ListC -> List representation function ****/
@@ -199,49 +173,69 @@ module Lists {
     ListConcAssoc(Rep(x), Rep(y), Rep(z));
   }
 
+  predicate AuxPreconditions(orig: List, x: ListC, y: List) 
+  {
+    (x.El? || x.Conc?) &&
+    (!x.Conc? ==> orig == Cons(x.val, y)) && 
+    (x.Conc? ==> InitDecomposableC(x)) && 
+    (!x.Conc? ==> ListConc(Rep(NilC), Cons(x.val, y)) == orig) && 
+    (x.Conc? ==> ListConc(Rep(x.left), Cons(x.right.val, y)) == orig)
+  }
+
+  lemma AuxProperty(orig: List, x: ListC, y: List) 
+    decreases y
+    requires x.El? || x.Conc?
+    requires !x.Conc? ==> orig == Cons(x.val, y) // Special case
+    requires x.Conc? ==> InitDecomposableC(x) // Structure of x 
+    requires !x.Conc? ==> ListConc(Rep(NilC), Cons(x.val, y)) == orig
+    requires x.Conc? ==> ListConc(Rep(x.left), Cons(x.right.val, y)) == orig 
+    ensures forall t: ListC :: (t in NewAux(orig, x, y) ==> ListConc(Rep(t.left), Rep(t.right)) == orig)
+  {
+    match y 
+    case Nil => {} 
+    case Cons(hd, tl) => {
+      RepAssociation(x, y);
+      AuxProperty(orig, Conc(x, El(hd)), tl);
+      var t := Conc(x, SimpleCoding(y));
+      SimpleRepInverse(y, SimpleCoding(y));
+      assert ListConc(Rep(t.left), Rep(t.right)) == orig;
+    }
+  }
+
+  lemma ListConcRightIdentity(a: List, b: List)
+    requires b == Nil 
+    ensures ListConc(a, b) == a 
+  {
+
+  }
+
   lemma RepAssociation(x: ListC, y: List)
     requires x.Conc? ==> InitDecomposableC(x)
     ensures x.Conc? ==> ListConc(Rep(x.left), Cons(x.right.val, y)) == ListConc(Rep(x), y) 
   {
-    assume x.Conc? ==> ListConc(Rep(x.left), Cons(x.right.val, y)) == ListConc(Rep(x), y);
+    // assume false;
+    match y 
+    case Nil => {
+      ListConcRightIdentity(Rep(x), y);
+    } 
+    case Cons(hd, tl) => {
+      
+    } 
   }
 
-  // lemma RepInverse(l: List, x: ListC) 
-  //   decreases x.left
-  //   requires x in NewComplex(l) && x != NilC
-  //   ensures Rep(x) == l
-  // {
-  //   // Base case
-  //   if !x.left.Conc? {
-  //     assert x == SimpleCoding(l);
-  //     SimpleRepInverse(l, x);
-  //   }
-  //   // Associate to the right 
-  //   else {
-  //     // x looks like ((init, El(a)), rest)
-  //     // If need the fact that x is InitDecomposable to prove the below, 
-  //     // uncomment the relevant facts about NewAux and NewComplex
-  //     assume Conc(x.left.left, Conc(x.left.right, x.right)) in NewComplex(l);
-  //     RepInverse(l, Conc(x.left.left, Conc(x.left.right, x.right)));
-  //     AssocRepEquiv(x.left.left, x.left.right, x.right);
-  //   }
-  // }
-
-  // lemma RepInverse(x: ListC, l: List)
-  //   requires x in NewComplex(l)
-  //   ensures Rep(x) == l
-  // {
-  //   match x 
-  //   case NilC => {}
-  //   case El(a) => {}
-  //   case Conc(a, b) => {
-  //     assert Rep(x) == ListConc(Rep(a), Rep(b));
-  //     assume a in NewComplex(Rep(a));
-  //     assume b in NewComplex(Rep(b));
-  //     // wts ListConc(Rep(a), Rep(b)) == l 
-  //     RepInverse(a, Rep(a)); RepInverse(b, Rep(b));
-  //   }
-  // }
+  lemma RepInverse(x: ListC, l: List)
+    requires x in NewComplex(l)
+    ensures Rep(x) == l
+  {
+    match x 
+    case NilC => {}
+    case El(a) => {}
+    case Conc(a, b) => {
+      assert Rep(x) == ListConc(Rep(a), Rep(b));
+      // This is really a statement about NewComplex
+      AuxProperty(l, El(l.head), l.tail); 
+    }
+  }
 
   // Sanity check
   method Main() {
@@ -250,13 +244,20 @@ module Lists {
     // var l := Nil;
     // var assoc := ComplexCoding(l);
     var assoc := NewComplex(l);
-    var c := assoc;
-    while c != {} 
-      decreases c;
+    // var c := assoc;
+    // while c != {} 
+    //   decreases c;
+    // {
+    //   var y :| y in c;
+    //   print PrintListC(y) + "\n";
+    //   c := c - { y };
+    // }
+    var i := 0;
+    while i < |assoc|
+      invariant i <= |assoc|
     {
-      var y :| y in c;
-      print PrintListC(y) + "\n";
-      c := c - { y };
+      print PrintListC(assoc[i]) + "\n";
+      i := i + 1;
     }
   }
 
